Properties/Liveness_tla.v
@@ -344,7 +344,7 @@ Lemma leads_to_exec_rel [e e' : exec World] (H : exec_rel e e')
   (P Q : World → Prop) (HP : World_rel_cong P) (HQ : World_rel_cong Q) :
   (e ⊨ ⌜ P ⌝ ~~> ⌜ Q ⌝) → (e' ⊨ ⌜ P ⌝ ~~> ⌜ Q ⌝).
 Proof.
-  unseal. pose proof (HP _ _ (H k)) as Htmp. rewrite <- Htmp in H1. saturate_assumptions!.
+  unseal. symmetry in H. pose proof (HP _ _ (H k)) as Htmp. saturate_assumptions!.
   destruct H0 as (k0 & H0). exists k0. eapply HQ. 2: apply H0. symmetry. apply H.
 Qed.
 
